
| Begriff             | Definition                                |
| ------------------- | ----------------------------------------- |
| Addition            | $(f(x) + g(x))' = f'(x) + g'(f)$          |
| Multiplikation      | $(a*f(x))'=a*f'(x)$                       |
| Produkteregel       | $(f*g)'=f'*g+f*g'$                        |
| Produkteregel mit 3 | $(f*g*h)'=f'*g*h+f*g'*h+f*g*h'$           |
| Kettenregel         | $(f(g(x)))'=f'(g(x))*g'(x)$               |
| Quotientenregel     | $({f \over g })' = {f'*g-f*g' \over g^2}$ |
 
